theory/x64EncodeProof.thy
@@ -3,11 +3,50 @@ imports
   Main
   rBPFCommType rBPFSyntax
   x64Assembler x64Disassembler
+  x64_encode_movl_rr_1
+  x64_encode_movl_rr_3
 begin
+
+declare if_split_asm [split]
+
 lemma x64_decode_encode_consistency:
-  "x64_decode pc l = Some (length l_bin, ins) \<Longrightarrow> (Some l_bin = x64_encode ins \<and> list_in_list l_bin pc l)"
+  "list_in_list l_bin pc l \<Longrightarrow> x64_decode pc l = Some (length l_bin, ins) \<Longrightarrow> Some l_bin = x64_encode ins"
   apply (cases ins; simp_all)
 
+  subgoal for dst src
+  \<comment> \<open> Pmovl_rr \<close> 
+    apply (unfold Let_def)
+    apply (unfold construct_rex_to_u8_def construct_modsib_to_u8_def)
+    apply (unfold x64_decode_def Let_def, auto simp add: split: option.splits)
+    subgoal
+      apply (cases l_bin, simp_all)
+      subgoal for l_bin1
+        apply (cases l_bin1, simp_all)
+        subgoal for t l_bin2
+          using encode_movl_rr_1 by blast
+        done
+      done
+
+    prefer 2
+      \<comment> \<open> prove False from context:
+      - rex = 0: `bitfield_insert_u8 3 (Suc 0) (bitfield_insert_u8 2 (Suc 0) (bitfield_insert_u8 (Suc 0) (Suc 0) (u8_of_bool (and (u8_of_ireg dst) 8 \<noteq> 0)) 0) (u8_of_bool (and (u8_of_ireg src) 8 \<noteq> 0))) 0 = 0`
+      - but src > 8: `and 1 (l ! pc >> 2) \<noteq> 0` \<close> 
+    subgoal
+      using encode_movl_rr_3 by blast
+
+    subgoal
+      done
+
+    done
+
+    subgoal
+
+      done
+
+    done
+
   done
+
+declare if_split_asm [split del]
 
 end
