theory/x64Syntax.thy
@@ -267,4 +267,8 @@ datatype instruction =
 
 type_synonym x64_asm = "instruction list"
 type_synonym x64_bin = "u8 list"
+
+lemma u8_of_ireg_of_u8_iff: "(u8_of_ireg r = i) = (ireg_of_u8 i = Some r)"
+  by (cases r, auto simp add: ireg_of_u8_def)
+
 end
