theory/x64_encode_movl_rr_1.thy
@@ -1,0 +1,186 @@
+theory x64_encode_movl_rr_1
+imports
+  Main
+  rBPFCommType rBPFSyntax
+  x64Syntax
+begin
+
+lemma encode_movl_rr_1_subgoal_1 [simp]: "n < 8 \<Longrightarrow> 
+  \<not> bit (192::int) n \<Longrightarrow> \<not> bit (7::int) n \<Longrightarrow> bit (56::int) n"
+  apply (cases n, simp_all)
+  subgoal for n1 apply (cases n1, simp_all)
+    subgoal for n2 apply (cases n2, simp_all)
+      subgoal for n3 apply (cases n3, simp_all)
+        subgoal for n4 apply (cases n4, simp_all)
+          subgoal for n5 apply (cases n5, simp_all)
+            subgoal for n6 apply (cases n6, simp_all)
+              done
+            done
+          done
+        done
+      done
+    done
+  done
+
+lemma encode_movl_rr_1_subgoal_2 [simp]: "n < 8 \<Longrightarrow> 
+  \<not> bit (192::int) n \<Longrightarrow> \<not> bit (7::int) n \<Longrightarrow> 3 \<le> n"
+  apply (cases n, simp_all)
+  subgoal for n1 apply (cases n1, simp_all)
+    subgoal for n2 apply (cases n2, simp_all)
+      done
+    done
+  done
+
+
+lemma encode_movl_rr_1_subgoal_3 [simp]: "n < 8 \<Longrightarrow> 
+  \<not> bit (192::int) n \<Longrightarrow> \<not> bit (7::int) n \<Longrightarrow> bit (71::int) n \<Longrightarrow> False"
+  apply (cases n, simp_all)
+  subgoal for n1 apply (cases n1, simp_all)
+    subgoal for n2 apply (cases n2, simp_all)
+      subgoal for n3 apply (cases n3, simp_all)
+        subgoal for n4 apply (cases n4, simp_all)
+          subgoal for n5 apply (cases n5, simp_all)
+            subgoal for n6 apply (cases n6, simp_all)
+              done
+            done
+          done
+        done
+      done
+    done
+  done
+
+lemma encode_movl_rr_1_subgoal_4 [simp]: "n < 8 \<Longrightarrow>
+  \<not> bit (192::int) n \<Longrightarrow> \<not> bit (56::int) n \<Longrightarrow> bit (8::int) n \<Longrightarrow> False"
+  apply (cases n, simp_all)
+  subgoal for n1 apply (cases n1, simp_all)
+    subgoal for n2 apply (cases n2, simp_all)
+      subgoal for n3 apply (cases n3, simp_all)
+        done
+      done
+    done
+  done
+
+lemma encode_movl_rr_1_subgoal_5 [simp]:
+  "\<not> bit (192::int) n \<Longrightarrow> \<not> 3 \<le> n \<Longrightarrow> bit (8::int) n \<Longrightarrow> False"
+  apply (cases n, simp_all)
+  subgoal for n1 apply (cases n1, simp_all)
+    subgoal for n2 apply (cases n2, simp_all)
+      done
+    done
+  done
+
+lemma encode_movl_rr_1_subgoal_6 [simp]:
+  "\<not> bit (192::int) n \<Longrightarrow> \<not> 3 \<le> n \<Longrightarrow> bit (56::int) n \<Longrightarrow> False"
+  apply (cases n, simp_all)
+  subgoal for n1 apply (cases n1, simp_all)
+    subgoal for n2 apply (cases n2, simp_all)
+      done
+    done
+  done
+
+lemma encode_movl_rr_1_subgoal_7 [simp]: "n < 8 \<Longrightarrow> bit (v::u8) n \<Longrightarrow>
+  \<not> bit (192::int) n \<Longrightarrow> bit (8::int) n \<Longrightarrow> bit v (3 + (n - 3))"
+  apply (cases n, simp_all)
+  subgoal for n1 apply (cases n1, simp_all)
+    subgoal for n2 apply (cases n2, simp_all)
+      subgoal for n3 apply (cases n3, simp_all)
+        using numeral_3_eq_3 by argo
+      done
+    done
+  done
+
+lemma encode_movl_rr_1_subgoal_8[simp]: "n < 8 \<Longrightarrow>
+  \<not> bit (192::int) n \<Longrightarrow> bit (8::int) n \<Longrightarrow> bit (71::int) n \<Longrightarrow> False"
+  apply (cases n, simp_all)
+  subgoal for n1 apply (cases n1, simp_all)
+    subgoal for n2 apply (cases n2, simp_all)
+      subgoal for n3 apply (cases n3, simp_all)
+        done
+      done
+    done
+  done
+
+lemma encode_movl_rr_1_subgoal_9 [simp]: "n < 8 \<Longrightarrow> bit (v::u8) n \<Longrightarrow>
+  \<not> bit (192::int) n \<Longrightarrow> bit (56::int) n \<Longrightarrow> bit v (3 + (n - 3))"
+  apply (cases n, simp_all)
+  subgoal for n1 apply (cases n1, simp_all)
+    subgoal for n2 apply (cases n2, simp_all)
+      subgoal for n3 apply (cases n3, simp_all)
+        subgoal using numeral_3_eq_3 by argo
+        subgoal for n4 apply (cases n4, simp_all)
+          subgoal
+            by (simp add: numeral_Bit0) 
+          subgoal for n5 apply (cases n5, simp_all)
+            by (simp add: eval_nat_numeral(3) numeral_Bit0)
+          done
+        done
+      done
+    done
+  done
+
+lemma encode_movl_rr_1_subgoal_10 [simp]: "n < 8 \<Longrightarrow>
+  \<not> bit (192::int) n \<Longrightarrow> bit (56::int) n \<Longrightarrow> bit (71::int) n \<Longrightarrow> False"
+  apply (cases n, simp_all)
+  subgoal for n1 apply (cases n1, simp_all)
+    subgoal for n2 apply (cases n2, simp_all)
+      subgoal for n3 apply (cases n3, simp_all)
+        subgoal for n4 apply (cases n4, simp_all)
+          subgoal for n5 apply (cases n5, simp_all)
+            done
+          done
+        done
+      done
+    done
+  done
+
+lemma and_3_shr_6_3_6 [simp]: "and 3 (v >> 6) = 3 \<Longrightarrow> bit v (Suc (Suc (Suc (Suc (Suc (Suc 0))))))"
+  by (metis Suc3_eq_add_3 bit_0 bit_and_iff bit_iff_odd_drop_bit bit_numeral_Bit1_0 numeral_3_eq_3 numeral_Bit0)
+
+lemma and_3_shr_6_3_7 [simp]: "and 3 ((v::u8) >> 6) = 3 \<Longrightarrow> bit v (Suc (Suc (Suc (Suc (Suc (Suc (Suc 0)))))))"
+  apply (simp add: bit_eq_iff)
+  apply (auto simp add: bit_simps)
+  apply (drule_tac x="1" in spec)
+  apply (simp add: eval_nat_numeral(2) eval_nat_numeral(3))
+  done
+
+
+lemma encode_movl_rr_1_subgoal_11 [simp]: "and 3 (v >> 6) = 3 \<Longrightarrow>
+  u8_of_ireg src = and (and 7 (v >> 3)) (- 9) \<Longrightarrow> u8_of_ireg dst = and (and 7 v) (- 9) \<Longrightarrow>
+  n < 8 \<Longrightarrow> bit (192::int) n \<Longrightarrow> bit v n"
+  apply (cases n, simp_all)
+  subgoal for n1 apply (cases n1, simp_all)
+    subgoal for n2 apply (cases n2, simp_all)
+      subgoal for n3 apply (cases n3, simp_all)
+        subgoal for n4 apply (cases n4, simp_all)
+          subgoal for n5 apply (cases n5, simp_all)
+            subgoal for n6 apply (cases n6, simp_all)
+              done
+            done
+          done
+        done
+      done
+    done
+  done
+
+
+lemma encode_movl_rr_1: "
+    and 3 (v >> 6) = 3 \<Longrightarrow>
+    ireg_of_u8 (bitfield_insert_u8 3 (Suc 0) (and 7 (v >> 3)) 0) = Some src \<Longrightarrow>
+    ireg_of_u8 (bitfield_insert_u8 3 (Suc 0) (and 7 v) 0) = Some dst \<Longrightarrow>
+    v = bitfield_insert_u8 6 2 (bitfield_insert_u8 3 3 (and 7 (u8_of_ireg dst)) (and 7 (u8_of_ireg src))) 3"
+  apply (simp add: u8_of_ireg_of_u8_iff[symmetric])
+  apply (unfold bitfield_insert_u8_def u8_of_bool_def Let_def)
+  apply simp
+  apply (rule bit_eqI)
+  subgoal for n
+    apply (simp add: bit_or_iff)
+    apply (auto simp add: bit_simps)
+    subgoal using encode_movl_rr_1_subgoal_3 by blast
+    subgoal using encode_movl_rr_1_subgoal_4 by blast
+    subgoal using encode_movl_rr_1_subgoal_5 by blast
+    subgoal using encode_movl_rr_1_subgoal_6 by blast
+    subgoal using encode_movl_rr_1_subgoal_8 by blast
+    subgoal using encode_movl_rr_1_subgoal_10 by blast
+    done
+  done
+end
